update merge sort

MergeSort.dfy
@@ -13,12 +13,18 @@ method MergeSort(a: array<int>) returns (b: array<int>)
 	ensures b.Length == a.Length && Sorted(b) && multiset(a[..]) == multiset(b[..])
 	decreases a.Length
 {
+	
 	b := new int[a.Length];
-	if(a.Length <= 1){
-		b := a;
+	//alternation
+	if(Guard1(a)){
+		assert Guard1(a);
+		b:=MS1(a,b);
+		
 	}
 	else{
 		
+		assert !Guard1(a); 
+
 		var mid := a.Length/2;
 
 		var leftSeq := a[0..mid];
@@ -39,9 +45,14 @@ method MergeSort(a: array<int>) returns (b: array<int>)
 
 		var leftSortedArr := MergeSort(leftArr);
 
+		assert leftSortedArr.Length == leftArr.Length && Sorted(leftSortedArr) && multiset(leftArr[..]) == multiset(leftSortedArr[..]);//post condition recursive call
+
 		assert multiset(a[..]) == multiset(leftArr[..])+multiset(rightArr[..]); // Still true after the assignment because MergeSort does not modify the given array
 		
 		var rightSortedArr := MergeSort(rightArr);
+
+		assert rightSortedArr.Length == rightArr.Length && Sorted(rightSortedArr) && multiset(rightArr[..]) == multiset(rightSortedArr[..]);//post condition recursive call
+
 
 		assert multiset(a[..]) == multiset(leftArr[..])+multiset(rightArr[..]); // Still true after the assignment because MergeSort does not modify the given array
 
@@ -58,44 +69,293 @@ method MergeSort(a: array<int>) returns (b: array<int>)
 	assert b.Length == a.Length && Sorted(b) && multiset(a[..]) == multiset(b[..]);
 }
 
+predicate method Guard1(a: array<int>)
+	requires 0<=a.Length
+{
+	a.Length <= 1
+}
+
+method MS1(a: array<int>,b0: array<int>) returns (b: array<int>)
+	 requires Guard1(a)
+
+	 ensures b.Length == a.Length && Sorted(b) && multiset(a[..]) == multiset(b[..])
+{	
+	assert  Guard1(a);
+	b:=b0;
+	// assignment
+	LemmaUpdateb(a,b);
+	b := a;
+	assert  b.Length == a.Length && Sorted(b) && multiset(a[..]) == multiset(b[..]);
+}
+
+lemma LemmaUpdateb(a: array<int>,b: array<int>)
+	requires Guard1(a)
+
+	ensures a.Length == a.Length && Sorted(a) && multiset(a[..]) == multiset(a[..])
+{}
+
 method Merge(b: array<int>, c: array<int>, d: array<int>)
 	requires b != c && b != d && b.Length == c.Length + d.Length
 	requires Sorted(c) && Sorted(d)
+
 	ensures Sorted(b) && multiset(b[..]) == multiset(c[..])+multiset(d[..])
 	modifies b
 {
-	var bi, ci, di := Loop1(b, c, d);
+	assert  b != c && b != d && b.Length == c.Length + d.Length;
+	assert Sorted(c) && Sorted(d);
+
+	var bi, ci, di := Loop1(b, c, d); // introduce local variable + strengthen postcondition
 	//==> 
 	assert ci == c.Length || di == d.Length;
+	Merga_alt(b, d, c, bi, di, ci);
 
-	if(ci == c.Length)
+	
+	assert Sorted(b) && multiset(b[..]) == multiset(c[..])+multiset(d[..]);
+}
+
+
+
+predicate method Guard2(ci:nat,c:array<int>)
+{
+	ci == c.Length
+} 
+
+method Merga_alt(b: array<int>, d: array<int>, c: array<int>, bi:nat, di:nat, ci:nat)
+	
+	requires  0 <= bi <= b.Length && 0 <= ci <= c.Length && 0 <= di <= d.Length
+	requires bi == ci+di
+	requires SortedSequence(b[0..bi]) && SortedSequence(c[..]) && SortedSequence(d[..])
+	requires multiset(b[..bi]) == multiset(c[..ci]) + multiset(d[..di])
+	requires ci == c.Length || di == d.Length
+	requires preffixASmallerThanSuffixB(b, c, bi, ci) && preffixASmallerThanSuffixB(b, d, bi, di)
+	requires b != c && b != d && b.Length == c.Length + d.Length
+	requires Sorted(c) && Sorted(d)
+
+	ensures Sorted(b) && multiset(b[..]) == multiset(c[..])+multiset(d[..])
+	modifies b;
+
 	{
-		Loop2(b, d, c, bi, di, ci);
+
+	assert  0 <= bi <= b.Length && 0 <= ci <= c.Length && 0 <= di <= d.Length;
+	assert bi == ci+di;
+	assert SortedSequence(b[0..bi]) && SortedSequence(c[..]) && SortedSequence(d[..]);
+	assert multiset(b[..bi]) == multiset(c[..ci]) + multiset(d[..di]);
+	assert ci == c.Length || di == d.Length;
+	assert preffixASmallerThanSuffixB(b, c, bi, ci) && preffixASmallerThanSuffixB(b, d, bi, di);
+	assert b != c && b != d && b.Length == c.Length + d.Length;
+	assert Sorted(c) && Sorted(d);
+
+	//alternation
+	if(Guard2(ci,c))
+	{
+		assert Guard2(ci,c);
+		Merga_alt_alt1(b, d, c, bi, di, ci);
+			
+			
 	}
 	else
 	{
+		assert !Guard2(ci,c);
 		assert di == d.Length;
-		Loop2(b, c, d, bi, ci, di);
+		Merga_alt_alt2(b, d, c, bi, di, ci);
+
 	}
 
 	assert Sorted(b) && multiset(b[..]) == multiset(c[..])+multiset(d[..]);
-}
+
+	}
+
+method Merga_alt_alt1(b: array<int>, d: array<int>, c: array<int>, bi:nat, di:nat, ci:nat) 
+
+	requires  0 <= bi <= b.Length && 0 <= ci <= c.Length && 0 <= di <= d.Length
+	requires bi == ci+di
+	requires SortedSequence(b[0..bi]) && SortedSequence(c[..]) && SortedSequence(d[..])
+	requires multiset(b[..bi]) == multiset(c[..ci]) + multiset(d[..di])
+	requires ci == c.Length || di == d.Length
+	requires preffixASmallerThanSuffixB(b, c, bi, ci) && preffixASmallerThanSuffixB(b, d, bi, di)
+	requires b != c && b != d && b.Length == c.Length + d.Length
+	requires Sorted(c) && Sorted(d)
+	requires Guard2(ci,c)
+
+	ensures Sorted(b) && multiset(b[..]) == multiset(c[..])+multiset(d[..])
+	modifies b;
+	{
+	assert  0 <= bi <= b.Length && 0 <= ci <= c.Length && 0 <= di <= d.Length;
+	assert bi == ci+di;
+	assert SortedSequence(b[0..bi]) && SortedSequence(c[..]) && SortedSequence(d[..]);
+	assert multiset(b[..bi]) == multiset(c[..ci]) + multiset(d[..di]);
+	assert ci == c.Length || di == d.Length;
+	assert preffixASmallerThanSuffixB(b, c, bi, ci) && preffixASmallerThanSuffixB(b, d, bi, di);
+	assert b != c && b != d && b.Length == c.Length + d.Length;
+	assert Sorted(c) && Sorted(d);
+	assert Guard2(ci,c);
+
+	Loop2(b, d, c, bi, di, ci);
+
+	assert Sorted(b) && multiset(b[..]) == multiset(c[..])+multiset(d[..]);
+	}
+
+method Merga_alt_alt2(b: array<int>, d: array<int>, c: array<int>, bi:nat, di:nat, ci:nat) 
+
+	requires  0 <= bi <= b.Length && 0 <= ci <= c.Length && 0 <= di <= d.Length
+	requires bi == ci+di
+	requires SortedSequence(b[0..bi]) && SortedSequence(c[..]) && SortedSequence(d[..])
+	requires multiset(b[..bi]) == multiset(c[..ci]) + multiset(d[..di])
+	requires ci == c.Length || di == d.Length
+	requires preffixASmallerThanSuffixB(b, c, bi, ci) && preffixASmallerThanSuffixB(b, d, bi, di)
+	requires b != c && b != d && b.Length == c.Length + d.Length
+	requires Sorted(c) && Sorted(d)
+	requires !Guard2(ci,c)
+
+	ensures Sorted(b) && multiset(b[..]) == multiset(c[..])+multiset(d[..])
+	modifies b;
+	{
+	assert  0 <= bi <= b.Length && 0 <= ci <= c.Length && 0 <= di <= d.Length;
+	assert bi == ci+di;
+	assert SortedSequence(b[0..bi]) && SortedSequence(c[..]) && SortedSequence(d[..]);
+	assert multiset(b[..bi]) == multiset(c[..ci]) + multiset(d[..di]);
+	assert ci == c.Length || di == d.Length;
+	assert preffixASmallerThanSuffixB(b, c, bi, ci) && preffixASmallerThanSuffixB(b, d, bi, di);
+	assert b != c && b != d && b.Length == c.Length + d.Length;
+	assert Sorted(c) && Sorted(d);
+	assert !Guard2(ci,c);
+
+	Loop2(b, c, d, bi, ci, di);
+
+	assert Sorted(b) && multiset(b[..]) == multiset(c[..])+multiset(d[..]);
+	}
+
+	
+
+
+
 
 method copySeqToArray(q:seq<int>, a:array<int>)
 	requires |q| == a.Length
 	ensures q == a[..]
 	modifies a
 {
-	var i:nat := 0;
+	assert |q| == a.Length;
 
-	while(i < a.Length)
-	invariant 0 <= i <= a.Length
-	invariant a[..i] == q[..i]
+	var i:nat; // introduce local variable + strengthen postcondition
+	i:=copySeqToArray_Help(q,a);
+	Lemma1(q,a,i);
+
+	assert q == a[..];
+	
+}
+
+lemma Lemma1(q:seq<int>, a:array<int>,i:nat)
+	requires Inv_copySeqToArray(q,a,i) && !Guard_Loop_copySeqToArray_Help(a,i)
+	ensures q == a[..]
+{}
+
+
+method copySeqToArray_Help(q:seq<int>, a:array<int>) returns (i:nat)
+	requires |q| == a.Length
+
+	ensures Inv_copySeqToArray(q,a,i) && !Guard_Loop_copySeqToArray_Help(a,i)
+	modifies a
+{
+
+	assert |q| == a.Length;
+
+	// sequential composition
+	i:=Init_copySeqToArray_Help(q,a);
+	i:=Loop_copySeqToArray_Help(q,a,i);
+
+	assert Inv_copySeqToArray(q,a,i) && !(i < a.Length);
+
+}
+
+method Loop_copySeqToArray_Help(q:seq<int>, a:array<int>,i0:nat) returns (i:nat)
+	requires |q| == a.Length
+	requires Inv_copySeqToArray(q,a,i0)
+
+	ensures Inv_copySeqToArray(q,a,i) &&  !Guard_Loop_copySeqToArray_Help(a,i)
+	modifies a
+{
+	assert  |q| == a.Length;
+	assert Inv_copySeqToArray(q,a,i0);
+
+	i:=i0;
+	// iteration
+	while(Guard_Loop_copySeqToArray_Help(a,i))
+	invariant Inv_copySeqToArray(q,a,i)
+	decreases a.Length-i
 	{
-
-		a[i] := q[i];
-		i := i+1;
+		i:=Loop_body_copySeqToArray_Help(q,a,i);
+		
 	}
+
+	assert Inv_copySeqToArray(q,a,i) &&  !Guard_Loop_copySeqToArray_Help(a,i);
+
+}
+
+predicate method Guard_Loop_copySeqToArray_Help(a:array<int>,i:nat)
+{
+	i < a.Length
+}
+
+
+method Loop_body_copySeqToArray_Help(q:seq<int>, a:array<int>,i0:nat) returns (i:nat)
+	requires |q| == a.Length 
+	requires Inv_copySeqToArray(q,a,i0) && Guard_Loop_copySeqToArray_Help(a,i0)
+
+	ensures Inv_copySeqToArray(q,a,i) && 0<=a.Length-i<a.Length-i0
+	ensures i0<i
+	modifies a
+{
+	assert |q| == a.Length ;
+	assert Inv_copySeqToArray(q,a,i0) && Guard_Loop_copySeqToArray_Help(a,i0);
+
+	i:=i0;
+	a[i] := q[i];
+	L_update(q,a,i);
+	i := i+1;//assignemnt
+
+	assert Inv_copySeqToArray(q,a,i) && 0<=a.Length-i<a.Length-i0;
+	assert i0<i;
+	
+
+}
+
+lemma L_update(q:seq<int>, a:array<int>,i:nat)
+	requires |q| == a.Length 
+	requires Inv_copySeqToArray(q,a,i) && Guard_Loop_copySeqToArray_Help(a,i)
+	requires a[i] ==q[i]
+
+	ensures Inv_copySeqToArray(q,a,i+1) && 0<=a.Length-(i+1)< a.Length-i
+	ensures i<i+1
+{}
+
+
+
+method Init_copySeqToArray_Help(q:seq<int>, a:array<int>) returns (i:nat)
+	requires |q| == a.Length
+
+	ensures Inv_copySeqToArray(q,a,i)
+{
+	assert |q| == a.Length;
+
+// assignment
+	LemmaInit_copySeqToArray_Help(q,a);
+	i:=0;
+
+	assert Inv_copySeqToArray(q,a,i);
+
+}
+
+lemma LemmaInit_copySeqToArray_Help(q: seq<int>,  a:array<int>)
+	requires |q| == a.Length
+
+	ensures Inv_copySeqToArray(q,a,0)
+{}
+
+predicate  Inv_copySeqToArray(q:seq<int>, a:array<int>,i:nat)
+reads a;
+{
+	0 <= i <= a.Length==|q| && a[..i] == q[..i]
 }
 
 method Loop1(b: array<int>, c: array<int>, d: array<int>) returns (bi:nat, ci:nat, di:nat)
@@ -111,31 +371,209 @@ method Loop1(b: array<int>, c: array<int>, d: array<int>) returns (bi:nat, ci:na
 
 	modifies b
 {
-	bi, ci, di := 0, 0, 0;
+	assert b != c && b != d && b.Length == c.Length + d.Length;
+	assert Sorted(c) && Sorted(d);
 
-	while(ci < c.Length && di < d.Length)
-		invariant LoopsInv(b, c, d, bi, ci, di)
+	bi, ci, di := Init_Loop1(b,c,d);
+	bi,ci,di:=Loop_Loop1(b,c,d,bi,ci,di);
+	lemama_end_loop1(b,c,d,bi,ci,di);
 
-		decreases c.Length-ci
-		decreases d.Length-di
+	assert  0 <= bi <= b.Length && 0 <= ci <= c.Length && 0 <= di <= d.Length;
+	assert bi == ci+di;
+	assert SortedSequence(b[0..bi]) && SortedSequence(c[..]) && SortedSequence(d[..]);
+	assert multiset(b[..bi]) == multiset(c[..ci]) + multiset(d[..di]);
+	assert ci == c.Length || di == d.Length;
+	assert preffixASmallerThanSuffixB(b, c, bi, ci) && preffixASmallerThanSuffixB(b, d, bi, di);
+
+	
+}
+
+lemma lemama_end_loop1(b: array<int>, c: array<int>, d: array<int>,bi:nat, ci:nat, di:nat)
+	requires !Guard_Loop1(c,d,ci,di) && LoopsInv(b, c, d, bi, ci, di)
+
+	ensures  0 <= bi <= b.Length && 0 <= ci <= c.Length && 0 <= di <= d.Length
+	ensures bi == ci+di
+	ensures SortedSequence(b[0..bi]) && SortedSequence(c[..]) && SortedSequence(d[..])
+	ensures multiset(b[..bi]) == multiset(c[..ci]) + multiset(d[..di])
+	ensures ci == c.Length || di == d.Length
+	ensures preffixASmallerThanSuffixB(b, c, bi, ci) && preffixASmallerThanSuffixB(b, d, bi, di)
+{}
+
+
+
+
+
+method Loop_Loop1(b: array<int>, c: array<int>, d: array<int>,bi0:nat, ci0:nat, di0:nat) returns(bi:nat, ci:nat, di:nat)
+	requires b != c && b != d && b.Length == c.Length + d.Length
+	requires Sorted(c) && Sorted(d)
+	requires LoopsInv(b, c, d, bi0, ci0, di0)
+
+	ensures  !Guard_Loop1(c,d,ci,di) && LoopsInv(b, c, d, bi, ci, di)
+	modifies b
 	{
-		
-		if(c[ci] <= d[di]){
-			
-			b[bi] := c[ci];
-			
-			ci := ci+1;
-		}
-		else{
-			
-			b[bi] := d[di];
-			
-			di := di+1;
-		}
 
+	assert b != c && b != d && b.Length == c.Length + d.Length;
+	assert Sorted(c) && Sorted(d);
+	assert LoopsInv(b, c, d, bi0, ci0, di0);
+
+	bi, ci, di:=bi0,ci0,di0;
+	//iterartion
+	while(Guard_Loop1(c,d,ci,di))
+	invariant LoopsInv(b, c, d, bi, ci, di)
+	decreases c.Length-ci 
+	decreases d.Length-di
+	{
+		// following assignment + contract frame
+		ci,di:=Loop_body_Loop1(b,c,d,bi,ci,di);
 		bi := bi+1;
 	}
+
+	assert !Guard_Loop1(c,d,ci,di) && LoopsInv(b, c, d, bi, ci, di);
+
+	}
+
+
+method Init_Loop1(b: array<int>, c: array<int>, d: array<int>) returns (bi:nat, ci:nat, di:nat)
+	requires b != c && b != d && b.Length == c.Length + d.Length
+	requires Sorted(c) && Sorted(d)
+
+	ensures LoopsInv(b, c, d, bi, ci, di)
+	{
+
+	assert b != c && b != d && b.Length == c.Length + d.Length;
+	assert Sorted(c) && Sorted(d);
+
+	// assignment
+	Lemma_Init_Loop1(b,c,d);
+	bi, ci, di:=0,0,0;
+
+	assert LoopsInv(b, c, d, bi, ci, di);
+
+	}
+
+lemma Lemma_Init_Loop1(b: array<int>, c: array<int>, d: array<int>) 
+	requires b != c && b != d && b.Length == c.Length + d.Length
+	requires Sorted(c) && Sorted(d)
+
+	ensures LoopsInv(b, c, d, 0,0,0)
+	{}
+
+
+
+predicate method Guard_Loop1(c: array<int>, d: array<int>,ci:nat, di:nat)
+	
+{
+	ci < c.Length && di < d.Length
 }
+
+method Loop_body_Loop1 (b: array<int>, c: array<int>, d: array<int>,bi:nat, ci0:nat, di0:nat) returns ( ci:nat, di:nat)
+	requires b != c && b != d && b.Length == c.Length + d.Length
+	requires Sorted(c) && Sorted(d)
+	requires LoopsInv(b, c, d, bi, ci0, di0 ) && Guard_Loop1(c,d,ci0,di0)
+
+	ensures LoopsInv(b, c, d, bi+1, ci, di) && (0<=c.Length - ci <= c.Length-ci0 && 0<=d.Length-di <= d.Length-di0)
+	modifies b;
+{
+
+	assert  b != c && b != d && b.Length == c.Length + d.Length;
+	assert Sorted(c) && Sorted(d);
+	assert LoopsInv(b, c, d, bi, ci0, di0 ) && Guard_Loop1(c,d,ci0,di0);
+
+	ci:=ci0;
+	di:=di0;
+	// alternation + contract frame (*2)
+	if(Guard_Loop_body_Loop1(c,d,ci,di)){
+		
+		assert Guard_Loop_body_Loop1(c,d,ci,di);
+		ci:=Loop_body_Loop1_update_ci(b,c,d,bi,ci,di);
+			
+	}
+	else{
+		
+		assert !Guard_Loop_body_Loop1(c,d,ci,di);
+		di:=Loop_body_Loop1_update_di(b,c,d,bi,ci,di);
+	}
+
+	assert LoopsInv(b, c, d, bi+1, ci, di) && (0<=c.Length - ci <= c.Length-ci0 && 0<=d.Length-di <= d.Length-di0);
+}
+
+predicate method Guard_Loop_body_Loop1(c: array<int>, d: array<int>,ci:nat, di:nat)
+	requires ci< c.Length
+	requires di< d.Length
+	reads c ,d 
+{
+	c[ci] <= d[di]
+}
+
+
+method Loop_body_Loop1_update_ci (b: array<int>, c: array<int>, d: array<int>,bi:nat, ci0:nat, di:nat) returns ( ci:nat)
+	requires b != c && b != d && b.Length == c.Length + d.Length
+	requires Sorted(c) && Sorted(d)
+	requires LoopsInv(b, c, d, bi, ci0, di) && Guard_Loop1(c,d,ci0,di) && Guard_Loop_body_Loop1(c,d,ci0,di)
+
+	ensures LoopsInv(b, c, d, bi+1, ci, di) && (0<=c.Length - ci < c.Length-ci0 && 0<=d.Length-di == d.Length-di)
+	ensures ci0<ci
+	modifies b
+{
+
+	assert b != c && b != d && b.Length == c.Length + d.Length;
+	assert Sorted(c) && Sorted(d);
+	assert LoopsInv(b, c, d, bi, ci0, di) && Guard_Loop1(c,d,ci0,di) && Guard_Loop_body_Loop1(c,d,ci0,di);
+	
+	ci:=ci0;
+	//assignemnt
+	b[bi] := c[ci];
+	LemmaUpdateci(b,c,d,bi,ci,di);
+	ci := ci+1;
+
+	assert LoopsInv(b, c, d, bi+1, ci, di) && (0<=c.Length - ci < c.Length-ci0 && 0<=d.Length-di == d.Length-di);
+	assert ci0<ci;
+
+}
+
+method Loop_body_Loop1_update_di (b: array<int>, c: array<int>, d: array<int>,bi:nat, ci:nat, di0:nat) returns ( di:nat)
+	requires b != c && b != d && b.Length == c.Length + d.Length
+	requires Sorted(c) && Sorted(d)
+	requires LoopsInv(b, c, d, bi, ci, di0) && Guard_Loop1(c,d,ci,di0) && !(Guard_Loop_body_Loop1(c,d,ci,di0))
+
+	ensures LoopsInv(b, c, d, bi+1, ci, di) && (0<=c.Length - ci == c.Length-ci && 0<=d.Length-di < d.Length-di0)
+	ensures di0<di
+	modifies b
+{
+	assert b != c && b != d && b.Length == c.Length + d.Length;
+	assert Sorted(c) && Sorted(d);
+	assert LoopsInv(b, c, d, bi, ci, di0) && Guard_Loop1(c,d,ci,di0) && !(Guard_Loop_body_Loop1(c,d,ci,di0));
+
+	di:=di0;
+	b[bi] := d[di];
+	LemmaUpdatedi(b,c,d,bi,ci,di);//assignemnt
+	di := di+1;
+
+	assert LoopsInv(b, c, d, bi+1, ci, di) && (0<=c.Length - ci == c.Length-ci && 0<=d.Length-di < d.Length-di0);
+	assert di0<di;
+
+}
+
+lemma LemmaUpdateci(b: array<int>, c: array<int>, d: array<int>,bi:nat, ci:nat, di:nat)
+	requires b != c && b != d && b.Length == c.Length + d.Length
+	requires Sorted(c) && Sorted(d)
+	requires LoopsInv(b, c, d, bi, ci, di) && Guard_Loop1(c,d,ci,di) && Guard_Loop_body_Loop1(c,d,ci,di)
+	requires b[bi] == c[ci];
+
+	ensures LoopsInv(b, c, d, bi+1, ci+1, di) && (0<=c.Length - (ci+1) < c.Length-ci) && (0<=d.Length-di == d.Length-di)
+	ensures ci<ci+1
+{}
+
+lemma LemmaUpdatedi(b: array<int>, c: array<int>, d: array<int>,bi:nat, ci:nat, di:nat)
+	requires b != c && b != d && b.Length == c.Length + d.Length
+	requires Sorted(c) && Sorted(d)
+	requires LoopsInv(b, c, d, bi, ci, di) && Guard_Loop1(c,d,ci,di) && !(Guard_Loop_body_Loop1(c,d,ci,di))
+	requires b[bi] == d[di]
+
+	ensures LoopsInv(b, c, d, bi+1, ci, di+1) &&  (0<=c.Length - ci == c.Length-ci && d.Length-di > d.Length-(di+1)>=0)
+	ensures di<di+1
+{}
+
 
 method Loop2(b: array<int>, arr1: array<int>, arr2: array<int>, bi0:nat, arr1i0:nat, arr2i0:nat) 
 	requires b.Length == arr1.Length + arr2.Length
@@ -151,17 +589,36 @@ method Loop2(b: array<int>, arr1: array<int>, arr2: array<int>, bi0:nat, arr1i0:
 
 	modifies b
 {
-	var bi, arr1i, arr2i := bi0, arr1i0, arr2i0;
 
-	while(arr1i < arr1.Length)
-		invariant LoopsInv(b, arr1, arr2, bi, arr1i, arr2i)
-	{		
-		b[bi] := arr1[arr1i];
+	assert b.Length == arr1.Length + arr2.Length;
+	assert 0 <= bi0 <= b.Length && 0 <= arr1i0 <= arr1.Length && 0 <= arr2i0 <= arr2.Length;
+	assert bi0 == arr1i0 + arr2i0;
+	assert SortedSequence(b[0..bi0]) && SortedSequence(arr1[..]) && SortedSequence(arr2[..]);
+	assert multiset(b[..bi0]) == multiset(arr1[..arr1i0]) + multiset(arr2[..arr2i0]);
+	assert arr2i0 == arr2.Length;
+	assert preffixASmallerThanSuffixB(b, arr1, bi0, arr1i0) && preffixASmallerThanSuffixB(b, arr2, bi0, arr2i0);
 
-		arr1i:= arr1i+1;
 
-		bi := bi+1;
-	}
+// introduce local variable + strengthen postcondition
+	var bi, arr1i, arr2i;
+	bi, arr1i, arr2i:=Loop2_help(b,arr1,arr2,bi0,arr1i0,arr2i0);
+	lemma_end_loop(b,arr1,arr2,bi,arr1i,arr2i);
+
+	assert Sorted(b);
+	assert multiset(b[..]) == multiset(arr1[..])+multiset(arr2[..]);
+
+}
+
+lemma lemma_end_loop(b: array<int>, arr1: array<int>, arr2: array<int>, bi:nat, arr1i:nat, arr2i:nat)
+	requires bi == b.Length;
+	requires  arr2i == arr2.Length
+	requires LoopsInv(b, arr1, arr2, bi, arr1i, arr2i) && !Guard_Loop2(arr1i,arr1) 
+
+	ensures  Sorted(b)
+	ensures multiset(b[..]) == multiset(arr1[..])+multiset(arr2[..])
+{
+	
+	assert  LoopsInv(b, arr1, arr2, bi, arr1i, arr2i) && !Guard_Loop2(arr1i,arr1) ;
 
 	assert arr2i == arr2.Length; // From pre-condition and the fact that the while loop didn't updated di
 	assert arr1i == arr1.Length; // From while inv "0 <= ci <= c.Length" + NOT(guard) "ci >= c.Length"
@@ -178,6 +635,189 @@ method Loop2(b: array<int>, arr1: array<int>, arr2: array<int>, bi0:nat, arr1i0:
 	// ==>
 	assert Sorted(b);
 }
+
+
+
+method Loop2_help(b: array<int>, arr1: array<int>, arr2: array<int>, bi0:nat, arr1i0:nat, arr2i0:nat) returns (bi:nat, arr1i:nat, arr2i:nat) 
+	requires b.Length == arr1.Length + arr2.Length
+	requires 0 <= bi0 <= b.Length && 0 <= arr1i0 <= arr1.Length && 0 <= arr2i0 <= arr2.Length
+	requires bi0 == arr1i0 + arr2i0
+	requires SortedSequence(b[0..bi0]) && SortedSequence(arr1[..]) && SortedSequence(arr2[..])
+	requires multiset(b[..bi0]) == multiset(arr1[..arr1i0]) + multiset(arr2[..arr2i0])
+	requires arr2i0 == arr2.Length
+	requires preffixASmallerThanSuffixB(b, arr1, bi0, arr1i0) && preffixASmallerThanSuffixB(b, arr2, bi0, arr2i0)
+
+
+	ensures LoopsInv(b, arr1, arr2, bi, arr1i, arr2i) && !Guard_Loop2(arr1i,arr1)
+	ensures  arr2i == arr2.Length
+
+	modifies b
+{
+	assert b.Length == arr1.Length + arr2.Length;
+	assert 0 <= bi0 <= b.Length && 0 <= arr1i0 <= arr1.Length && 0 <= arr2i0 <= arr2.Length;
+	assert bi0 == arr1i0 + arr2i0;
+	assert SortedSequence(b[0..bi0]) && SortedSequence(arr1[..]) && SortedSequence(arr2[..]);
+	assert multiset(b[..bi0]) == multiset(arr1[..arr1i0]) + multiset(arr2[..arr2i0]);
+	assert arr2i0 == arr2.Length;
+	assert preffixASmallerThanSuffixB(b, arr1, bi0, arr1i0) && preffixASmallerThanSuffixB(b, arr2, bi0, arr2i0);
+	
+	// sequential composition
+	bi, arr1i, arr2i:=Init_Loop2(b,arr1,arr2,bi0,arr1i0,arr2i0);
+	bi, arr1i, arr2i:=Loop_Loop2(b,arr1,arr2,bi,arr1i, arr2i);
+
+	assert LoopsInv(b, arr1, arr2, bi, arr1i, arr2i) && !Guard_Loop2(arr1i,arr1);
+	assert  arr2i == arr2.Length;
+
+
+}
+
+
+method Loop_Loop2(b: array<int>, arr1: array<int>, arr2: array<int>, bi0:nat, arr1i0:nat, arr2i0:nat)returns (bi:nat, arr1i:nat, arr2i:nat) 
+	requires b.Length == arr1.Length + arr2.Length
+	requires 0 <= bi0 <= b.Length && 0 <= arr1i0 <= arr1.Length && 0 <= arr2i0 <= arr2.Length
+	requires bi0 == arr1i0 + arr2i0
+	requires SortedSequence(b[0..bi0]) && SortedSequence(arr1[..]) && SortedSequence(arr2[..])
+	requires multiset(b[..bi0]) == multiset(arr1[..arr1i0]) + multiset(arr2[..arr2i0])
+	requires arr2i0 == arr2.Length
+	requires preffixASmallerThanSuffixB(b, arr1, bi0, arr1i0) && preffixASmallerThanSuffixB(b, arr2, bi0, arr2i0)
+	requires LoopsInv(b, arr1, arr2, bi0, arr1i0, arr2i0)
+
+	ensures LoopsInv(b, arr1, arr2, bi, arr1i, arr2i) && !Guard_Loop2(arr1i,arr1)
+	ensures  arr2i == arr2.Length
+
+	modifies b;
+{
+	assert b.Length == arr1.Length + arr2.Length;
+	assert 0 <= bi0 <= b.Length && 0 <= arr1i0 <= arr1.Length && 0 <= arr2i0 <= arr2.Length;
+	assert bi0 == arr1i0 + arr2i0;
+	assert SortedSequence(b[0..bi0]) && SortedSequence(arr1[..]) && SortedSequence(arr2[..]);
+	assert multiset(b[..bi0]) == multiset(arr1[..arr1i0]) + multiset(arr2[..arr2i0]);
+	assert arr2i0 == arr2.Length;
+	assert preffixASmallerThanSuffixB(b, arr1, bi0, arr1i0) && preffixASmallerThanSuffixB(b, arr2, bi0, arr2i0);
+	assert LoopsInv(b, arr1, arr2, bi0, arr1i0, arr2i0);
+
+		
+	bi,arr1i,arr2i:=bi0,arr1i0,arr2i0;
+	//iteration
+	while(Guard_Loop2(arr1i,arr1))
+	invariant LoopsInv(b, arr1, arr2, bi, arr1i, arr2i)
+	decreases arr1.Length-arr1i
+	{		
+		
+		bi,arr1i:=Loop_Loop2_Body(b, arr1, arr2, bi, arr1i, arr2i);
+	}
+
+	assert LoopsInv(b, arr1, arr2, bi, arr1i, arr2i) && !Guard_Loop2(arr1i,arr1);
+	assert  arr2i == arr2.Length; 
+
+}
+
+predicate method Guard_Loop2(arr1i:nat,arr1: array<int>)
+{
+	arr1i < arr1.Length
+}
+
+method Loop_Loop2_Body(b: array<int>, arr1: array<int>, arr2: array<int>, bi0:nat, arr1i0:nat, arr2i0:nat)returns (bi:nat, arr1i:nat)
+	requires b.Length == arr1.Length + arr2.Length
+	requires 0 <= bi0 <= b.Length && 0 <= arr1i0 <= arr1.Length && 0 <= arr2i0 <= arr2.Length
+	requires bi0 == arr1i0 + arr2i0
+	requires SortedSequence(b[0..bi0]) && SortedSequence(arr1[..]) && SortedSequence(arr2[..])
+	requires multiset(b[..bi0]) == multiset(arr1[..arr1i0]) + multiset(arr2[..arr2i0])
+	requires arr2i0 == arr2.Length
+	requires preffixASmallerThanSuffixB(b, arr1, bi0, arr1i0) && preffixASmallerThanSuffixB(b, arr2, bi0, arr2i0)
+	requires LoopsInv(b, arr1, arr2, bi0, arr1i0, arr2i0) && Guard_Loop2(arr1i0,arr1)
+
+	ensures LoopsInv(b, arr1, arr2, bi, arr1i, arr2i0) && 0<=arr1.Length-arr1i< arr1.Length-arr1i0 
+	ensures arr1i0<arr1i
+	ensures bi>bi0
+	modifies b;
+{
+	assert b.Length == arr1.Length + arr2.Length;
+	assert 0 <= bi0 <= b.Length && 0 <= arr1i0 <= arr1.Length && 0 <= arr2i0 <= arr2.Length;
+	assert bi0 == arr1i0 + arr2i0;
+	assert SortedSequence(b[0..bi0]) && SortedSequence(arr1[..]) && SortedSequence(arr2[..]);
+	assert multiset(b[..bi0]) == multiset(arr1[..arr1i0]) + multiset(arr2[..arr2i0]);
+	assert arr2i0 == arr2.Length;
+	assert preffixASmallerThanSuffixB(b, arr1, bi0, arr1i0) && preffixASmallerThanSuffixB(b, arr2, bi0, arr2i0);
+	assert LoopsInv(b, arr1, arr2, bi0, arr1i0, arr2i0) && Guard_Loop2(arr1i0,arr1);
+
+		
+	bi,arr1i:=bi0,arr1i0;
+	b[bi] := arr1[arr1i];
+	Lemma_as_Loop_Loop2_Body(b,arr1,arr2,bi0,arr1i0,arr2i0);
+	arr1i:= arr1i+1;
+	bi := bi+1;
+
+	assert LoopsInv(b, arr1, arr2, bi, arr1i, arr2i0) && 0<=arr1.Length-arr1i< arr1.Length-arr1i0 ;
+	assert arr1i0<arr1i;
+	assert bi>bi0;
+
+}
+
+lemma Lemma_as_Loop_Loop2_Body(b: array<int>, arr1: array<int>, arr2: array<int>, bi0:nat, arr1i0:nat, arr2i0:nat)
+	requires b.Length == arr1.Length + arr2.Length
+	requires 0 <= bi0 <= b.Length && 0 <= arr1i0 <= arr1.Length && 0 <= arr2i0 <= arr2.Length
+	requires bi0 == arr1i0 + arr2i0
+	requires SortedSequence(b[0..bi0]) && SortedSequence(arr1[..]) && SortedSequence(arr2[..])
+	requires multiset(b[..bi0]) == multiset(arr1[..arr1i0]) + multiset(arr2[..arr2i0])
+	requires arr2i0 == arr2.Length
+	requires preffixASmallerThanSuffixB(b, arr1, bi0, arr1i0) && preffixASmallerThanSuffixB(b, arr2, bi0, arr2i0)
+	requires LoopsInv(b, arr1, arr2, bi0, arr1i0, arr2i0) && Guard_Loop2(arr1i0,arr1)
+	requires b[bi0] == arr1[arr1i0];
+
+	ensures LoopsInv(b, arr1, arr2, bi0+1, arr1i0+1, arr2i0) && 0<=arr1.Length-(arr1i0+1)< arr1.Length-arr1i0 
+	ensures arr1i0<arr1i0+1
+	ensures bi0+1>bi0
+{}
+
+
+
+
+method Init_Loop2(b: array<int>, arr1: array<int>, arr2: array<int>, bi0:nat, arr1i0:nat, arr2i0:nat)returns (bi:nat, arr1i:nat, arr2i:nat) 
+	requires b.Length == arr1.Length + arr2.Length
+	requires 0 <= bi0 <= b.Length && 0 <= arr1i0 <= arr1.Length && 0 <= arr2i0 <= arr2.Length
+	requires bi0 == arr1i0 + arr2i0
+	requires SortedSequence(b[0..bi0]) && SortedSequence(arr1[..]) && SortedSequence(arr2[..])
+	requires multiset(b[..bi0]) == multiset(arr1[..arr1i0]) + multiset(arr2[..arr2i0])
+	requires arr2i0 == arr2.Length
+	requires preffixASmallerThanSuffixB(b, arr1, bi0, arr1i0) && preffixASmallerThanSuffixB(b, arr2, bi0, arr2i0)
+
+	ensures bi==bi0 && arr1i==arr1i0 &&  arr2i==arr2i0 
+	ensures arr2i == arr2.Length
+	ensures LoopsInv(b, arr1, arr2, bi, arr1i, arr2i)
+	 
+	{
+
+	assert b.Length == arr1.Length + arr2.Length;
+	assert 0 <= bi0 <= b.Length && 0 <= arr1i0 <= arr1.Length && 0 <= arr2i0 <= arr2.Length;
+	assert bi0 == arr1i0 + arr2i0;
+	assert SortedSequence(b[0..bi0]) && SortedSequence(arr1[..]) && SortedSequence(arr2[..]);
+	assert multiset(b[..bi0]) == multiset(arr1[..arr1i0]) + multiset(arr2[..arr2i0]);
+	assert arr2i0 == arr2.Length;
+	assert preffixASmallerThanSuffixB(b, arr1, bi0, arr1i0) && preffixASmallerThanSuffixB(b, arr2, bi0, arr2i0);
+
+	LemmaInit_Loop2(b,arr1,arr2,bi0,arr1i0,arr2i0);
+	bi, arr1i, arr2i := bi0, arr1i0, arr2i0;
+
+	assert bi==bi0 && arr1i==arr1i0 &&  arr2i==arr2i0 ;
+	assert arr2i == arr2.Length;
+	assert LoopsInv(b, arr1, arr2, bi, arr1i, arr2i);
+
+	}
+
+
+lemma LemmaInit_Loop2(b: array<int>, arr1: array<int>, arr2: array<int>, bi0:nat, arr1i0:nat, arr2i0:nat)
+	requires b.Length == arr1.Length + arr2.Length
+	requires 0 <= bi0 <= b.Length && 0 <= arr1i0 <= arr1.Length && 0 <= arr2i0 <= arr2.Length
+	requires bi0 == arr1i0 + arr2i0
+	requires SortedSequence(b[0..bi0]) && SortedSequence(arr1[..]) && SortedSequence(arr2[..])
+	requires multiset(b[..bi0]) == multiset(arr1[..arr1i0]) + multiset(arr2[..arr2i0])
+	requires arr2i0 == arr2.Length
+	requires preffixASmallerThanSuffixB(b, arr1, bi0, arr1i0) && preffixASmallerThanSuffixB(b, arr2, bi0, arr2i0)
+
+	ensures arr2i0 == arr2.Length
+	ensures LoopsInv(b, arr1, arr2, bi0, arr1i0, arr2i0)
+{}
 
 predicate LoopsInv(b: array<int>, arr1: array<int>, arr2: array<int>, bi:nat, arr1i:nat, arr2i:nat)
 	reads b, arr1, arr2
